Commutative mrdts -> new interface

new/App_comm_mrdts.fsti
@@ -30,11 +30,16 @@ val eq_is_equiv (a b:concrete_st)
 // operation type
 val app_op_t : eqtype
 
-type timestamp_t = pos
+type timestamp_t = pos 
 
-type op_t = timestamp_t & app_op_t
+type op_t = timestamp_t & (nat (*replica ID*) & app_op_t)
 
 type log = seq op_t
+
+let get_rid (_,(rid,_)) = rid
+
+let mem_rid (rid:nat) (l:log) =
+  exists e. mem e l /\ fst (snd e) = rid
 
 unfold
 let ( ++ ) (l1 l2:log) = Seq.append l1 l2
@@ -54,217 +59,203 @@ type st0 = concrete_st & erased log
 let v_of (s:st0) : concrete_st = fst s
 let ops_of (s:st0) : GTot log = snd s
 
+//pre-condition for do
+val do_pre (s:concrete_st) (o:op_t) : prop
+
 // apply an operation to a state
-val do (s:concrete_st) (o:op_t) : concrete_st
+val do (s:concrete_st) (o:op_t{do_pre s o}) : concrete_st
 
 val lem_do (a b:concrete_st) (op:op_t)
-   : Lemma (requires eq a b)
-           (ensures eq (do a op) (do b op))
+   : Lemma (requires eq a b /\ do_pre a op)
+           (ensures do_pre b op /\ eq (do a op) (do b op))
 
+let rec do_pre_prop (x:concrete_st) (l:log) : Tot prop (decreases length l) =
+  match length l with
+  |0 -> True
+  |_ -> do_pre x (head l) /\ do_pre_prop (do x (head l)) (tail l)
+  
 // applying a log of operations to a concrete state
-let rec apply_log (x:concrete_st) (l:log) : Tot concrete_st (decreases length l) =
+let rec apply_log (x:concrete_st) (l:log{do_pre_prop x l}) : Tot concrete_st (decreases length l) =
   match length l with
   |0 -> x
   |_ -> apply_log (do x (head l)) (tail l)                   
 
 // property of apply_log
 let rec lem_apply_log (x:concrete_st) (l:log)
-  : Lemma (ensures (length l > 0 ==> apply_log x l == do (apply_log x (fst (un_snoc l))) (last l)))
+  : Lemma (requires do_pre_prop x l)
+          (ensures (length l > 0 ==> do_pre_prop x (fst (un_snoc l)) /\ do_pre (apply_log x (fst (un_snoc l))) (last l) /\ 
+                                    (apply_log x l == apply_log (do x (head l)) (tail l)) /\
+                                    (apply_log x l == do (apply_log x (fst (un_snoc l))) (last l))) /\
+                   (length l = 0 ==> apply_log x l == x))
           (decreases length l) =
   match length l with
   |0 -> ()
   |_ -> lem_apply_log (do x (head l)) (tail l)
 
-type st1 = s:st0{(v_of s == apply_log init_st (ops_of s))}
+type st1 = s:st0{do_pre_prop init_st (ops_of s) /\ (v_of s == apply_log init_st (ops_of s))}
 
 let valid_st (s:st0) : prop =
   distinct_ops (ops_of s) /\
+  do_pre_prop init_st (ops_of s) /\
   (v_of s == apply_log init_st (ops_of s))
 
 type st = s:st0{valid_st s}
 
-type resolve_conflict_res =
-  | First_then_second //o2.o1 
-  | Second_then_first //o1.o2
-
-val resolve_conflict (x:op_t) (y:op_t{fst x <> fst y}) : resolve_conflict_res
+//pre-condition for merge
+val merge_pre (l a b:concrete_st) : prop
 
 // concrete merge operation
-val concrete_merge (lca s1 s2:concrete_st) : Tot concrete_st
+val merge (l a:concrete_st) (b:concrete_st{merge_pre l a b}) : Tot concrete_st
 
+// returns the inverse state by undoing the last operation
+#push-options "--z3rlimit 50"
 let inverse_st (s:st{Seq.length (ops_of s) > 0}) 
-  : GTot (i:st{(v_of s == do (v_of i) (last (ops_of s))) /\
-               (ops_of i = fst (un_snoc (ops_of s))) /\
-               (ops_of s = snoc (ops_of i) (last (ops_of s))) /\
-               is_prefix (ops_of i) (ops_of s) /\
-               (forall id. mem_id id (ops_of i) <==> mem_id id (ops_of s) /\ id <> fst (last (ops_of s)))}) =
-  let p,_ = un_snoc (ops_of s) in
-  let r = apply_log init_st p in
+  : GTot (i:st{(let _, last2 = un_snoc (ops_of s) in
+               do_pre (v_of i) (last (ops_of s)) /\
+               s == (do (v_of i) last2, hide (snoc (ops_of i) last2))) /\
+               (forall id. mem_id id (ops_of i) <==> mem_id id (ops_of s) /\ id <> fst (last (ops_of s)))}) = 
   lem_apply_log init_st (ops_of s);
   let p, l = un_snoc (ops_of s) in
   let r = apply_log init_st p in
   lemma_split (ops_of s) (length (ops_of s) - 1); 
   lemma_append_count_assoc_fst p (snd (split (ops_of s) (length (ops_of s) - 1))); 
-  distinct_invert_append p (snd (split (ops_of s) (length (ops_of s) - 1)));
+  distinct_invert_append p (snd (split (ops_of s) (length (ops_of s) - 1))); 
   (r, hide p)
 
-//currently present in App.fsti as Log MRDT needs it
-let rec inverse_helper (s:concrete_st) (l':log) (op:op_t)
-  : Lemma (ensures (let l = Seq.snoc l' op in 
-                   (apply_log s l == do (apply_log s l') op))) 
-          (decreases length l')
-  = Seq.un_snoc_snoc l' op;
-    match length l' with
-    |0 -> ()
-    |_ -> inverse_helper (do s (head l')) (tail l') op
-
-//currently present in App.fsti as Log MRDT needs it
 let rec split_prefix (s:concrete_st) (l:log) (a:log)
-  : Lemma (requires is_prefix l a)
-          (ensures (apply_log s a == apply_log (apply_log s l) (diff a l)) /\
+  : Lemma (requires is_prefix l a /\ do_pre_prop s a)
+          (ensures do_pre_prop s l /\ do_pre_prop (apply_log s l) (diff a l) /\ 
+                   (apply_log s a == apply_log (apply_log s l) (diff a l)) /\
                    (forall e. mem e l ==> mem e a) /\
                    (Seq.length a > Seq.length l ==> (last a) == (last (diff a l))))
           (decreases Seq.length l)
   = match Seq.length l with
     |0 -> ()
+    |1 -> ()
     |_ -> split_prefix (do s (head l)) (tail l) (tail a)
 
-let consistent_branches (lca s1 s2:st1) =
-  distinct_ops (ops_of lca) /\ distinct_ops (ops_of s1) /\ distinct_ops (ops_of s2) /\
-  is_prefix (ops_of lca) (ops_of s1) /\
-  is_prefix (ops_of lca) (ops_of s2) /\
-  (forall id id1. mem_id id (ops_of lca) /\ mem_id id1 (diff (ops_of s1) (ops_of lca)) ==> lt id id1) /\
-  (forall id id1. mem_id id (ops_of lca) /\ mem_id id1 (diff (ops_of s2) (ops_of lca)) ==> lt id id1) /\
-  (forall id. mem_id id (diff (ops_of s1) (ops_of lca)) ==> not (mem_id id (diff (ops_of s2) (ops_of lca))))
+let cons_reps (l a b:st1) =
+  distinct_ops (ops_of l) /\ distinct_ops (ops_of a) /\ distinct_ops (ops_of b) /\
+  is_prefix (ops_of l) (ops_of a) /\
+  is_prefix (ops_of l) (ops_of b) /\
+  (forall id. mem_id id (diff (ops_of a) (ops_of l)) ==> not (mem_id id (diff (ops_of b) (ops_of l)))) /\
+  (forall rid. mem_rid rid (diff (ops_of a) (ops_of l)) ==> ~ (mem_rid rid (diff (ops_of b) (ops_of l))))
 
-let consistent_branches_s1_gt0 (lca s1 s2:st1) =
-  consistent_branches lca s1 s2 /\
-  length (ops_of s1) > length (ops_of lca)
+let cons_reps_a_gt0 (l a b:st1) =
+  cons_reps l a b /\
+  length (ops_of a) > length (ops_of l)
 
-let consistent_branches_s2_gt0 (lca s1 s2:st1) =
-  consistent_branches lca s1 s2 /\
-  length (ops_of s2) > length (ops_of lca)
+let cons_reps_b_gt0 (l a b:st1) =
+  cons_reps l a b /\
+  length (ops_of b) > length (ops_of l)
 
-let consistent_branches_s1s2_gt0 (lca s1 s2:st1) =
-  consistent_branches lca s1 s2 /\
-  length (ops_of s1) > length (ops_of lca) /\
-  length (ops_of s2) > length (ops_of lca)
+let cons_reps_ab_gt0 (l a b:st1) =
+  cons_reps l a b /\
+  length (ops_of a) > length (ops_of l) /\
+  length (ops_of b) > length (ops_of l)
 
-let do_st (s:st1) (o:op_t) : st1 =
+//currently present in App.fsti as Log MRDT needs it
+let rec inverse_helper (s:concrete_st) (l':log) (op:op_t)
+  : Lemma (requires do_pre_prop s l' /\ do_pre (apply_log s l') op)
+          (ensures (let l = Seq.snoc l' op in 
+                   do_pre_prop s l /\ 
+                   (apply_log s l == do (apply_log s l') op)))
+          (decreases length l') // [SMTPat (do_pre_prop s l' /\ do_pre (apply_log s l') op)] 
+  = Seq.un_snoc_snoc l' op;
+    match length l' with
+    |0 -> ()
+    |_ -> inverse_helper (do s (head l')) (tail l') op
+
+let cons_reps_a'b' (l a b:st)
+  : Lemma (requires cons_reps_ab_gt0 l a b)
+          (ensures cons_reps l (inverse_st a) (inverse_st b)) =
+  lem_inverse (ops_of l) (ops_of a);
+  lem_inverse (ops_of l) (ops_of b);
+  inverse_diff_id_s1'_s2' (ops_of l) (ops_of a) (ops_of b);
+  assume (forall rid. mem_rid rid (diff (ops_of (inverse_st a)) (ops_of l)) ==> 
+                 ~ (mem_rid rid (diff (ops_of (inverse_st b)) (ops_of l)))); ()
+
+let cons_reps_b' (l a b:st)
+  : Lemma (requires cons_reps_b_gt0 l a b)
+          (ensures cons_reps l a (inverse_st b)) =
+  lem_inverse (ops_of l) (ops_of b);
+  split_prefix init_st (ops_of l) (ops_of (inverse_st b));
+  inverse_diff_id_s2' (ops_of l) (ops_of a) (ops_of b);
+  assume (forall rid. mem_rid rid (diff (ops_of a) (ops_of l)) ==> 
+                 ~ (mem_rid rid (diff (ops_of (inverse_st b)) (ops_of l)))); ()
+
+let cons_reps_a' (l a b:st)
+  : Lemma (requires cons_reps_a_gt0 l a b)
+          (ensures cons_reps l (inverse_st a) b) =
+  lem_inverse (ops_of l) (ops_of a);
+  split_prefix init_st (ops_of l) (ops_of (inverse_st a));
+  inverse_diff_id_s1' (ops_of l) (ops_of a) (ops_of b);
+  assume (forall rid. mem_rid rid (diff (ops_of (inverse_st a)) (ops_of l)) ==> 
+                 ~ (mem_rid rid (diff (ops_of b) (ops_of l)))); ()
+                 
+let do_st (s:st1) (o:op_t{do_pre (v_of s) o}) : st1 =
+  inverse_helper init_st (ops_of s) o;
   split_prefix init_st (ops_of s) (snoc (ops_of s) o); 
   (do (v_of s) o, hide (snoc (ops_of s) o))
 
-// Prove that merge is commutative
-val merge_is_comm (lca s1 s2:st)
-  : Lemma (requires consistent_branches lca s1 s2)
-          (ensures (eq (concrete_merge (v_of lca) (v_of s1) (v_of s2)) 
-                       (concrete_merge (v_of lca) (v_of s2) (v_of s1)))) 
+/////////////////////////////////////////////////////////////////////////////
 
-val linearizable_s1_0''_base_base (lca s1 s2':st) (last2:op_t)
-  : Lemma (requires consistent_branches lca s1 (do_st s2' last2) /\
-                    ops_of s1 = ops_of lca /\ ops_of s2' = ops_of lca /\
-                    length (ops_of lca) = 0)
-        
-          (ensures eq (do (v_of s2') last2) (concrete_merge (v_of lca) (v_of s1) (do (v_of s2') last2)))
+val merge_comm (l a b:st)
+  : Lemma (requires cons_reps l a b /\ merge_pre (v_of l) (v_of a) (v_of b))
+          (ensures merge_pre (v_of l) (v_of b) (v_of a) /\
+                   (eq (merge (v_of l) (v_of a) (v_of b)) 
+                       (merge (v_of l) (v_of b) (v_of a)))) 
 
-val linearizable_s1_0''_base_ind (lca s1 s2':st) (last2:op_t)
-  : Lemma (requires consistent_branches lca s1 (do_st s2' last2) /\
-                    ops_of s1 = ops_of lca /\ ops_of s2' = ops_of lca /\
-                    length (ops_of lca) > 0 /\
+val merge_idem (s:st)
+  : Lemma (requires merge_pre (v_of s) (v_of s) (v_of s))
+          (ensures eq (merge (v_of s) (v_of s) (v_of s)) (v_of s))
 
-                    (let l' = inverse_st lca in
-                    let s1' = inverse_st s1 in
-                    let s2'' = inverse_st s2' in
-                    consistent_branches l' s1' (do_st s2'' last2) /\
-                    ops_of s1' = ops_of l' /\ ops_of s2'' = ops_of l' /\
-                    eq (do (v_of s2'') last2) (concrete_merge (v_of l') (v_of s1') (do (v_of s2'') last2))))
+val fast_fwd (a b:st)
+  : Lemma (requires cons_reps a a b /\ merge_pre (v_of a) (v_of a) (v_of b))
+          (ensures eq (merge (v_of a) (v_of a) (v_of b)) (v_of b))
 
-          (ensures eq (do (v_of s2') last2) (concrete_merge (v_of lca) (v_of s1) (do (v_of s2') last2)))
+val lin_prop1 (s:concrete_st) (op1 op2:op_t)
+  : Lemma (requires do_pre s op1 /\ do_pre s op2 /\ do_pre (do s op1) op2 /\ do_pre (do s op2) op1)
+          (ensures eq (do (do s op1) op2) (do (do s op2) op1))
 
-val linearizable_s1_0''_ind (lca s1 s2':st) (last2:op_t)
-  : Lemma (requires consistent_branches lca s1 (do_st s2' last2) /\
-                    ops_of s1 = ops_of lca /\
-                    length (ops_of s2') > length (ops_of lca) /\
+val lin_prop3 (l a b:concrete_st) (last2:op_t) 
+  :  Lemma (requires do_pre b last2 /\ merge_pre l a b /\ merge_pre l a (do b last2) /\
+                     do_pre (merge l a b) last2)
+           (ensures eq (do (merge l a b) last2) (merge l a (do b last2)))
 
-                    (let inv2 = inverse_st s2' in
-                    consistent_branches lca s1 (do_st inv2 last2) /\
-                    eq (do (v_of inv2) last2) (concrete_merge (v_of lca) (v_of s1) (do (v_of inv2) last2))))
-        
-          (ensures eq (do (v_of s2') last2) (concrete_merge (v_of lca) (v_of s1) (do (v_of s2') last2)))
+val inter_merge1 (l:concrete_st) (o1 o2 o3:op_t)
+  : Lemma (requires fst o1 <> fst o3 /\ fst o2 <> fst o3 /\ 
+                    do_pre l o1 /\ do_pre l o3 /\ do_pre (do l o1) o2 /\ do_pre (do l o3) o1 /\ do_pre (do (do l o3) o1) o2 /\
+                    merge_pre (do l o1) (do (do l o1) o2) (do (do l o3) o1))
+          (ensures eq (merge (do l o1) (do (do l o1) o2) (do (do l o3) o1)) (do (do (do l o3) o1) o2))
 
-val linearizable_s1_0_s2_0_base (lca s1 s2:st)
-  : Lemma (requires consistent_branches lca s1 s2 /\
-                    ops_of s1 == ops_of lca /\ ops_of s2 == ops_of lca)       
-          (ensures eq (v_of lca) (concrete_merge (v_of lca) (v_of s1) (v_of s2)))
-          
-val linearizable_gt0_base (lca s1 s2:st) (last1 last2:op_t)
-  : Lemma (requires consistent_branches lca (do_st s1 last1) (do_st s2 last2) /\
-                    consistent_branches lca s1 s2 /\
-                    ops_of s1 = ops_of lca /\ ops_of s2 = ops_of lca /\
-                    fst last1 <> fst last2)
-         
-          (ensures (First_then_second? (resolve_conflict last1 last2) ==>
-                      (eq (do (concrete_merge (v_of lca) (v_of s1) (do (v_of s2) last2)) last1)
-                          (concrete_merge (v_of lca) (do (v_of s1) last1) (do (v_of s2) last2)))) /\
+val inter_merge2 (l s s':concrete_st) (o1 o2 o3:op_t)
+  : Lemma (requires fst o2 <> fst o3 /\ fst o1 <> fst o3 /\
+                    do_pre l o3 /\ do_pre l o2 /\ do_pre s' o2 /\ do_pre s o2 /\
+                    merge_pre l s (do l o3) /\ merge_pre s (do s o2) s' /\
+                    eq (merge l s (do l o3)) s' /\
+                    eq (merge s (do s o2) s') (do s' o2) /\
+                    do_pre s o1 /\ do_pre s' o1 /\ do_pre (do s o1) o2 /\ do_pre (do s' o1) o2 /\
+                    merge_pre (do s o1) (do (do s o1) o2) (do s' o1))
+          (ensures eq (merge (do s o1) (do (do s o1) o2) (do s' o1)) (do (do s' o1) o2))
 
-                   (Second_then_first? (resolve_conflict last1 last2) ==>
-                      (eq (do (concrete_merge (v_of lca) (do (v_of s1) last1) (v_of s2)) last2)
-                          (concrete_merge (v_of lca) (do (v_of s1) last1) (do (v_of s2) last2)))))                 
+val inter_merge3 (l a b c:concrete_st) (op op':op_t) 
+  : Lemma (requires merge_pre l a b /\ eq (merge l a b) c /\
+                    (forall (o:op_t). do_pre b o /\ do_pre c o /\ merge_pre l a (do b o) ==> eq (merge l a (do b o)) (do c o)) /\
+                    do_pre b op /\ do_pre c op /\ do_pre (do b op) op' /\ do_pre (do c op) op' /\
+                    merge_pre l a (do (do b op) op'))
+          (ensures eq (merge l a (do (do b op) op')) (do (do c op) op'))
 
-val linearizable_gt0_ind (lca s1 s2:st) (last1 last2:op_t)
-  : Lemma (requires consistent_branches lca (do_st s1 last1) (do_st s2 last2) /\
-                    consistent_branches lca s1 s2 /\
-                    length (ops_of s2) > length (ops_of lca) /\
-                    fst last1 <> fst last2)
-       
-          (ensures (let s2' = inverse_st s2 in
-                   ((First_then_second? (resolve_conflict last1 last2) /\
-                    consistent_branches lca s1 (do_st s2' last2) /\
-                    consistent_branches lca (do_st s1 last1) (do_st s2' last2) /\
-                    consistent_branches lca s1 (do_st s2 last2) /\
-                    eq (do (concrete_merge (v_of lca) (v_of s1) (do (v_of s2') last2)) last1)
-                       (concrete_merge (v_of lca) (do (v_of s1) last1) (do (v_of s2') last2))) ==>
-                   
-                    (eq (do (concrete_merge (v_of lca) (v_of s1) (do (v_of s2) last2)) last1)
-                        (concrete_merge (v_of lca) (do (v_of s1) last1) (do (v_of s2) last2)))) /\
-                          
-                   ((ops_of s1 = ops_of lca /\
-                    Second_then_first? (resolve_conflict last1 last2) /\
-                    consistent_branches lca (do_st s1 last1) s2' /\
-                    consistent_branches lca (do_st s1 last1) (do_st s2' last2) /\
-                    consistent_branches lca (do_st s1 last1) s2 /\
-                    eq (do (concrete_merge (v_of lca) (do (v_of s1) last1) (v_of s2')) last2)
-                       (concrete_merge (v_of lca) (do (v_of s1) last1) (do (v_of s2') last2))) ==>
-                   
-                    (eq (do (concrete_merge (v_of lca) (do (v_of s1) last1) (v_of s2)) last2)
-                        (concrete_merge (v_of lca) (do (v_of s1) last1) (do (v_of s2) last2))))))
-                       
-val linearizable_gt0_ind1 (lca s1 s2:st) (last1 last2:op_t)
-  : Lemma (requires consistent_branches lca (do_st s1 last1) (do_st s2 last2) /\
-                    consistent_branches lca s1 s2 /\
-                    length (ops_of s1) > length (ops_of lca) /\
-                    fst last1 <> fst last2)
-                           
-          (ensures (let s1' = inverse_st s1 in
-                   ((ops_of s2 = ops_of lca /\
-                    First_then_second? (resolve_conflict last1 last2) /\
-                    consistent_branches lca s1' (do_st s2 last2) /\
-                    consistent_branches lca (do_st s1' last1) (do_st s2 last2) /\
-                    consistent_branches lca s1 (do_st s2 last2) /\
-                    eq (do (concrete_merge (v_of lca) (v_of s1') (do (v_of s2) last2)) last1)
-                       (concrete_merge (v_of lca) (do (v_of s1') last1) (do (v_of s2) last2))) ==>
-                    eq (do (concrete_merge (v_of lca) (v_of s1) (do (v_of s2) last2)) last1)
-                       (concrete_merge (v_of lca) (do (v_of s1) last1) (do (v_of s2) last2))) /\
-
-                   ((Second_then_first? (resolve_conflict last1 last2) /\
-                    consistent_branches lca (do_st s1' last1) s2 /\
-                    consistent_branches lca (do_st s1' last1) (do_st s2 last2) /\
-                    consistent_branches lca (do_st s1 last1) s2 /\
-                    eq (do (concrete_merge (v_of lca) (do (v_of s1') last1) (v_of s2)) last2)
-                       (concrete_merge (v_of lca) (do (v_of s1') last1) (do (v_of s2) last2)) ==>
-                    eq (do (concrete_merge (v_of lca) (do (v_of s1) last1) (v_of s2)) last2)
-                       (concrete_merge (v_of lca) (do (v_of s1) last1) (do (v_of s2) last2))))))
-                       
+val inter_merge4 (l s:concrete_st) (o1 o2 o3 o4:op_t)
+  : Lemma (requires fst o1 <> fst o3 /\ fst o1 <> fst o4 /\ fst o2 <> fst o3 /\
+                    do_pre l o1 /\ do_pre s o3 /\ do_pre (do l o1) o2 /\ do_pre (do s o3) o1 /\ do_pre (do (do s o3) o1) o2 /\
+                    merge_pre (do l o1) (do (do l o1) o2) (do (do s o3) o1) /\
+                    eq (merge (do l o1) (do (do l o1) o2) (do (do s o3) o1)) (do (do (do s o3) o1) o2) /\
+                    do_pre s o4 /\ do_pre (do s o4) o3 /\ do_pre (do (do s o4) o3) o1 /\ do_pre (do (do (do s o4) o3) o1) o2 /\
+                    merge_pre (do l o1) (do (do l o1) o2) (do (do (do s o4) o3) o1))
+          (ensures eq (merge (do l o1) (do (do l o1) o2) (do (do (do s o4) o3) o1)) 
+                      (do (do (do (do s o4) o3) o1) o2))
+                      
 ////////////////////////////////////////////////////////////////
 //// Sequential implementation //////
 
@@ -286,62 +277,7 @@ val initial_eq (_:unit)
 
 //equivalence between states of sequential type and MRDT at every operation
 val do_eq (st_s:concrete_st_s) (st:concrete_st) (op:op_t)
-  : Lemma (requires eq_sm st_s st)
+  : Lemma (requires eq_sm st_s st /\ do_pre st op)
           (ensures eq_sm (do_s st_s op) (do st op))
 
-////////////////////////////////////////////////////////////////
-//// Linearization properties //////
-
-val conv_prop1 (s:concrete_st) (op1 op2:op_t)
-  : Lemma (eq (do (do s op1) op2) (do (do s op2) op1))
-
-val conv_prop2 (lca s1 s2:concrete_st) (op:op_t) 
-  : Lemma (eq (do (concrete_merge lca s1 s2) op) (concrete_merge lca (do s1 op) s2))
-
-val conv_prop3 (lca s1 s2:concrete_st) (op:op_t) 
-  :  Lemma (eq (do (concrete_merge lca s1 s2) op) (concrete_merge lca s1 (do s2 op)))
-
-val conv_prop4 (s:concrete_st)
-  : Lemma (eq (concrete_merge s s s) s)
-
-val conv_prop5 (lca s1 s2:concrete_st) (op:op_t)
-  : Lemma (eq (concrete_merge lca (do s1 op) (do s2 op)) (do (do (concrete_merge lca s1 s2) op) op))
-
-////////////////////////////////////////////////////////////////
-//// Linearization properties - intermediate merge //////
-
-val inter_prop1 (l:concrete_st) (o1 o2 o3:op_t)
-  : Lemma (requires fst o1 <> fst o3 /\ fst o2 <> fst o3 /\ 
-                    resolve_conflict o1 o3 = First_then_second /\
-                    resolve_conflict o2 o3 = First_then_second)
-          (ensures eq (concrete_merge (do l o1) (do (do l o1) o2) (do (do l o3) o1)) (do (do (do l o3) o1) o2))
-
-val inter_prop2 (s s':concrete_st) (o1 o2:op_t) 
-  : Lemma (requires eq (concrete_merge s (do s o2) s') (do s' o2))
-          (ensures eq (concrete_merge (do s o1) (do (do s o1) o2) (do s' o1)) (do (do s' o1) o2))
-
-val inter_prop3 (l a b c:concrete_st) (op op':op_t)
-  : Lemma (requires eq (concrete_merge l a b) c /\ 
-                    (forall (o:op_t). eq (concrete_merge l a (do b o)) (do c o)))
-          (ensures eq (concrete_merge l a (do (do b op) op')) (do (do c op) op'))
-
-val inter_prop4 (l s:concrete_st) (o1 o2 o3 o3':op_t)
-  : Lemma (requires fst o1 <> fst o3 /\ fst o2 <> fst o3 /\
-                    resolve_conflict o1 o3 = First_then_second /\
-                    resolve_conflict o2 o3 = First_then_second /\
-                    eq (concrete_merge (do l o1) (do (do l o1) o2) (do (do s o3) o1)) (do (do (do s o3) o1) o2))
-          (ensures eq (concrete_merge (do l o1) (do (do l o1) o2) (do (do (do s o3') o3) o1)) 
-                      (do (do (do (do s o3') o3) o1) o2))
-
-////////////////////////////////////////////////////////////////
-//// Recursive merge condition //////
-
-val rec_merge (s si si' sn sn':concrete_st)
-  : Lemma (requires eq (concrete_merge s sn sn') (concrete_merge si sn (concrete_merge s si sn')) /\
-                    eq (concrete_merge s sn sn') (concrete_merge si' sn' (concrete_merge s sn si')) /\
-                    eq (concrete_merge s sn si') (concrete_merge si sn (concrete_merge s si si')) /\
-                    eq (concrete_merge s si sn') (concrete_merge si' sn' (concrete_merge s si' si)))         
-          (ensures (eq (concrete_merge s sn sn')
-                       (concrete_merge (concrete_merge s si si') (concrete_merge s si sn') (concrete_merge s si' sn))))
-          
 ////////////////////////////////////////////////////////////////
