new/commutative_mrdts/Rga_set/App_comm_mrdts.fst
@@ -1,23 +1,30 @@
 module App_comm_mrdts
 
-module M = Map_extended
-module S = FStar.Set
+module S = Set_extended_new
 
 #set-options "--query_stats"
+let unique_st (s:S.t (nat & (nat & nat))) =
+  forall e. S.mem e s ==> ~ (exists e1. S.mem e1 s /\ snd e <> snd e1 /\ fst e = fst e1)
+
+let mem_id_s (id:nat) (s:S.t (nat & (nat & nat))) 
+  : (r:bool {s = S.empty ==> r == false}) =
+  S.exists_s s (fun e -> fst e = id)
 
 // the concrete state type
-// It is a list of unique elements
-type concrete_st = M.t nat (S.set nat)
+type concrete_st = s:(S.t (nat & (nat & nat)) & S.t nat) {unique_st (fst s) /\ (forall id. S.mem id (snd s) ==> mem_id_s id (fst s))}
+                   // first ele of the pair is a tuple of timestamp, 
+                   //     id after which the ele is to be inserted and ele to be inserted
+                   // second ele of the pair is a tombstone set
 
-//initial state
-let init_st = M.const S.empty
+// init state
+let init_st : concrete_st = (S.empty, S.empty)
 
-let sel (s:concrete_st) k = if M.contains s k then M.sel s k else S.empty
-
+// equivalence between 2 concrete states
 let eq (a b:concrete_st) =
-  (forall id. M.contains a id = M.contains b id /\
-         S.equal (sel a id) (sel b id))
+  S.equal (fst a) (fst b) /\
+  S.equal (snd a) (snd b)
 
+// few properties of equivalence relation
 let symmetric (a b:concrete_st) 
   : Lemma (requires eq a b)
           (ensures eq b a) = ()
@@ -31,53 +38,69 @@ let eq_is_equiv (a b:concrete_st)
           (ensures eq a b) = ()
           
 // operation type
-// (the only operation is Add, so nat * nat is fine)
-type app_op_t = nat * nat
+type app_op_t:eqtype = 
+  |Add_after : after_id:nat -> ele:nat -> app_op_t //inserts ele after after_id
+  |Remove : id:pos -> app_op_t //removes the element with identifier id
 
-let key (op:op_t) = fst (snd op)
+let get_ele (op:op_t{Add_after? (snd (snd op))}) : nat =
+  let (_, (_, Add_after _ ele)) = op in ele
 
-let value (op:op_t) = snd (snd op)
+let get_after_id (op:op_t{Add_after? (snd (snd op))}) : nat =
+  let (_, (_, Add_after id _)) = op in id
 
+let get_rem_id (op:op_t{Remove? (snd (snd op))}) : pos =
+  let (_, (_, Remove id)) = op in id
+  
 //pre-condition for do
-let do_pre (s:concrete_st) (o:op_t) : prop = true
+let do_pre (s:concrete_st) (o:op_t) : prop = 
+  match o with
+  |(ts, (_, Add_after after_id ele)) -> ~ (mem_id_s ts (fst s)) /\ (~ (after_id = 0) ==> mem_id_s after_id (fst s))
+  |(_, (_, Remove id)) -> mem_id_s id (fst s)
 
-let do (s:concrete_st) (op:op_t{do_pre s op}) =
-  let (ts, (_, (k,v))) = op in
-  M.upd s k (S.union (S.singleton v) (sel s k))
-
-#push-options "--ifuel 3"
+// apply an operation to a state
+let do (s:concrete_st) (o:op_t{do_pre s o}) : concrete_st =
+  match o with
+  |(ts, (_, Add_after after_id ele)) -> (S.insert (ts, (after_id, ele)) (fst s), snd s)
+  |(_, (_, Remove id)) -> (fst s, S.insert id (snd s))
+  
 let lem_do (a b:concrete_st) (op:op_t)
    : Lemma (requires eq a b /\ do_pre a op)
-           (ensures do_pre b op /\ eq (do a op) (do b op)) = ()
-
+           (ensures eq (do a op) (do b op)) = ()
+           
 //pre-condition for merge
-let merge_pre (l a b:concrete_st) : prop = true
+let merge_pre (l a b:concrete_st) : prop = 
+  (forall id. mem_id_s id (fst l) ==> ~ (mem_id_s id (S.difference (fst a) (fst l)))) /\
+  (forall id. mem_id_s id (fst l) ==> ~ (mem_id_s id (S.difference (fst b) (fst l)))) /\
+  (forall id. mem_id_s id (S.difference (fst a) (fst l)) ==> ~ (mem_id_s id (S.difference (fst b) (fst l))))
 
 // concrete merge operation
 let merge (l a:concrete_st) (b:concrete_st{merge_pre l a b}) : concrete_st =
-  let keys = S.union (M.domain l) (S.union (M.domain a) (M.domain b)) in
-  let u:concrete_st = M.const_on keys S.empty in
-  M.iter_upd (fun k v -> S.union (sel l k) (S.union (sel a k) (sel b k))) u
+  (S.union (fst l) (S.union (fst a) (fst b)),   
+   S.union (snd l) (S.union (snd a) (snd b)))
 
 let merge_comm (l a b:st)
   : Lemma (requires cons_reps l a b /\ merge_pre (v_of l) (v_of a) (v_of b))
           (ensures merge_pre (v_of l) (v_of b) (v_of a) /\
                    (eq (merge (v_of l) (v_of a) (v_of b)) 
                        (merge (v_of l) (v_of b) (v_of a)))) = ()
- 
+         
 let merge_idem (s:st)
   : Lemma (requires merge_pre (v_of s) (v_of s) (v_of s))
           (ensures eq (merge (v_of s) (v_of s) (v_of s)) (v_of s)) = ()
 
+#push-options "--z3rlimit 50 --ifuel 3"
 let rec fast_fwd (a b:st)
   : Lemma (requires cons_reps a a b /\ merge_pre (v_of a) (v_of a) (v_of b))
-          (ensures eq (merge (v_of a) (v_of a) (v_of b)) (v_of b)) 
+          (ensures S.subset (fst (v_of a)) (fst (v_of b)) /\
+                   S.subset (snd (v_of a)) (snd (v_of b)) /\
+                   eq (merge (v_of a) (v_of a) (v_of b)) (v_of b)) 
           (decreases length (ops_of b)) =
   if ops_of a = ops_of b then ()
   else 
     (let b' = inverse_st b in
      cons_reps_b' a a b;
      fast_fwd a b')
+
 
 let lin_prop1 (s:concrete_st) (op1 op2:op_t)
   : Lemma (requires do_pre s op1 /\ do_pre s op2 /\ do_pre (do s op1) op2 /\ do_pre (do s op2) op1)
@@ -113,32 +136,28 @@ let inter_merge3 (l a b c:concrete_st) (op op':op_t)
 
 let inter_merge4 (l s:concrete_st) (o1 o2 o3 o4:op_t)
   : Lemma (requires fst o1 <> fst o3 /\ fst o1 <> fst o4 /\ fst o2 <> fst o3 /\
-                    eq (merge (do l o1) (do (do l o1) o2) (do (do s o3) o1)) (do (do (do s o3) o1) o2))
-          (ensures eq (merge (do l o1) (do (do l o1) o2) (do (do (do s o4) o3) o1)) 
-                      (do (do (do (do s o4) o3) o1) o2)) = admit()
-                      
-let inter_merge41 (l s:concrete_st) (o1 o2 o3 o4:op_t)
-  : Lemma (requires (exists a b. eq (merge l a b) s) /\ //extra 
-                    fst o1 <> fst o3 /\ fst o1 <> fst o4 /\ fst o2 <> fst o3 /\
-                    eq (merge (do l o1) (do (do l o1) o2) (do (do s o3) o1)) (do (do (do s o3) o1) o2))
+                    do_pre l o1 /\ do_pre s o3 /\ do_pre (do l o1) o2 /\ do_pre (do s o3) o1 /\ do_pre (do (do s o3) o1) o2 /\
+                    merge_pre (do l o1) (do (do l o1) o2) (do (do s o3) o1) /\
+                    eq (merge (do l o1) (do (do l o1) o2) (do (do s o3) o1)) (do (do (do s o3) o1) o2) /\
+                    do_pre s o4 /\ do_pre (do s o4) o3 /\ do_pre (do (do s o4) o3) o1 /\ do_pre (do (do (do s o4) o3) o1) o2 /\
+                    merge_pre (do l o1) (do (do l o1) o2) (do (do (do s o4) o3) o1))
           (ensures eq (merge (do l o1) (do (do l o1) o2) (do (do (do s o4) o3) o1)) 
                       (do (do (do (do s o4) o3) o1) o2)) = ()
-                     
+
 ////////////////////////////////////////////////////////////////
 //// Sequential implementation //////
 
 // the concrete state 
-type concrete_st_s = concrete_st
+type concrete_st_s = admit()
 
 // init state 
-let init_st_s = init_st
+let init_st_s = admit()
 
 // apply an operation to a state 
-let do_s (s:concrete_st_s) (op:op_t) : concrete_st_s = 
-  do s op
+let do_s (s:concrete_st_s) (op:op_t) : concrete_st_s = admit()
 
 //equivalence relation between the concrete states of sequential type and MRDT
-let eq_sm (st_s:concrete_st_s) (st:concrete_st) = st_s == st
+let eq_sm (st_s:concrete_st_s) (st:concrete_st) = admit()
 
 //initial states are equivalent
 let initial_eq _
@@ -147,6 +166,6 @@ let initial_eq _
 //equivalence between states of sequential type and MRDT at every operation
 let do_eq (st_s:concrete_st_s) (st:concrete_st) (op:op_t)
   : Lemma (requires eq_sm st_s st /\ do_pre st op)
-          (ensures eq_sm (do_s st_s op) (do st op)) = ()
+          (ensures eq_sm (do_s st_s op) (do st op)) = admit()
 
 ////////////////////////////////////////////////////////////////
